Let's first simplify the given expression ( y = \frac{4x}{x \cdot xy} + 9 ).

The expression can be broken down as follows:

Simplify $$( \frac{4x}{x \cdot xy} )$$

Next, we'll simplify $$( y = 6x + 4 )$$.

Let's solve it step by step.
Expression 1: $$( y = \frac{4x}{x \cdot xy} + 9 )$$

First, we can simplify the fraction:
$$[ \frac{4x}{x \cdot xy} = \frac{4x}{x^2 y} ]$$

It simplifies further to:
$$[ \frac{4}{xy} ]$$

Therefore, the simplified form of the expression $( y = \frac{4x}{x \cdot xy} + 9 )$ is:
$$[ y = \frac{4}{xy} + 9 ]$$
Expression 2: $$( y = 6x + 4 )$$

This expression is already simplified. To reaffirm:

$$[ y = 6x + 4 ]$$

To summarize, the simplified form of the given mathematical expressions are:

$$( y = \frac{4}{xy} + 9 )$$
$$( y = 6x + 4 )$$

If you have any specific questions or need further assistance, feel free to ask!
